Refinery/Term/Extrinsic/Refinement.lean
@@ -1,1 +1,66 @@
 import Refinery.Term.Extrinsic.Typing
+
+namespace Refinery
+
+namespace Term
+
+abbrev RWS (φ α ε) := Ctx? α ε → Ty α → Term φ (Ty α) → Term φ (Ty α) → Prop
+
+variable {φ : Type u} {α : Type v} {ε : Type w} [S : Signature φ α ε]
+
+class RWS.IsWt (R : RWS φ α ε) : Prop where
+  left_wt {Γ A a b} (hab : R Γ A a b) : Term.IsWt ⊤ Γ A a
+  right_wt {Γ A a b} (hab : R Γ A a b) : Term.IsWt ⊤ Γ A b
+
+theorem RWS.IsWt.mk' (R : RWS φ α ε)
+  (both_wt : ∀ {Γ A a b}, R Γ A a b → Term.IsWt ⊤ Γ A a ∧ Term.IsWt ⊤ Γ A b)
+  : R.IsWt where
+  left_wt hab := (both_wt hab).left
+  right_wt hab := (both_wt hab).right
+
+inductive RWS.cc (R : RWS φ α ε) : RWS φ α ε
+  | base {Γ A a b} : R Γ A a b → cc R Γ A a b
+  | refl {Γ e a A} : (Γ ⊢[e] a : A) → cc R Γ A a a
+  | symm {Γ a b A} : cc R Γ A a b → cc R Γ A b a
+  | trans {Γ a b c A} : cc R Γ A a b → cc R Γ A b c → cc R Γ A a c
+  | let₁ {Γ Γl Γr A B a b a' b'} :
+    Γ.PSSplit Γl Γr →
+    cc R Γr A a a' → cc R (Γl.cons ⟨A, ⊤, ⊥⟩) B b b'
+      → cc R Γ B (.let₁ a A b) (.let₁ a' A b')
+  | let₂ {Γ Γl Γr A B C a b a' b'} :
+    Γ.PSSplit Γl Γr →
+    cc R Γr (.tensor A B) a a' → cc R ((Γl.cons ⟨A, ⊤, ⊥⟩).cons ⟨B, ⊤, ⊥⟩) C b b'
+      → cc R Γ C (.let₂ a A B b) (.let₂ a' A B b')
+  | pair {Γ Γl Γr A B a b a' b'} :
+    Γ.PSSplit Γl Γr →
+    cc R Γl A a a' → cc R Γr B b b' → cc R Γ (.tensor A B) (.pair a b) (.pair a' b')
+  | inl {Γ A B a a'} : cc R Γ A a a' → cc R Γ (.coprod A B) (.inl A B a) (.inl A B a')
+  | inr {Γ A B b b'} : cc R Γ B b b' → cc R Γ (.coprod A B) (.inr A B b) (.inr A B b')
+  | abort {Γ A a a'} : cc R Γ .empty a a' → cc R Γ A (.abort A a) (.abort A a')
+  | iter {Γ Γl Γr A B a b a' b'} :
+    Γ.PSSplit Γl Γr →
+    Γl.copy → Γl.del →
+    cc R Γr A a a' →
+    cc R (Γl.cons ⟨A, ⊤, ⊥⟩) (.coprod B A) b b' →
+    cc R Γ B (.iter a A B b) (.iter a' A B b')
+
+theorem RWS.cc.wt {R : RWS φ α ε} [RWS.IsWt R] {Γ A a a'} (h : cc R Γ A a a')
+  : Term.IsWt ⊤ Γ A a ∧ Term.IsWt ⊤ Γ A a' := by induction h with
+  | base R => exact ⟨IsWt.left_wt R, IsWt.right_wt R⟩
+  | refl => constructor <;> apply Deriv.wt_top <;> assumption
+  | _ =>
+    simp only [Term.IsWt] at *
+    cases_type* And Nonempty
+    constructor <;> constructor
+    <;> first | assumption | (constructor <;> first | exact S.top_iterative | assumption)
+
+instance RWS.cc.instWt (R : RWS φ α ε) [RWS.IsWt R] : RWS.IsWt (RWS.cc R) where
+  left_wt h := (RWS.cc.wt h).left
+  right_wt h := (RWS.cc.wt h).right
+
+inductive Rewrite : RWS φ α ε
+  | let_op {Γ Γl Γr A B C a c} :
+    Γ.PSSplit Γl Γr → S.IsFn f e A B → (Γr ⊢[⊤] a : A) → (Γl.cons ⟨B, ⊤, ⊥⟩ ⊢[⊤] c : C) →
+    Rewrite Γ C (.let₁ (.op f a) A c) (.let₁ a A (.let₁ (.op f (.bv 0)) B (↑¹ c)))
+  -- | let_let₁ {Γ Γc Γl Γm Γr} :
+  --   Γ.PSSplit Γc Γr → Γc.PSSplit Γl Γm → Rewrite R _ _ .invalid .invalid
