Refinery/Term/Extrinsic/Typing.lean
@@ -14,15 +14,15 @@ inductive Deriv : ε → Ctx? α ε → Ty α → Term φ (Ty α) → Type _
   | bv {Γ} : Γ.At ⟨A, 1, e⟩ n → Deriv e Γ A (.bv n)
   | op {Γ e A B f a} : S.IsFn f e A B → Deriv e Γ A a → Deriv e Γ B (.op f a)
   | let₁ {Γ Γl Γr e A B a b} :
-    Γ.PSSplit Γr Γl →
-    Deriv e Γl A a → Deriv e (Γr.cons ⟨A, ⊤, ⊥⟩) B b → Deriv e Γ B (.let₁ a A b)
+    Γ.PSSplit Γl Γr →
+    Deriv e Γr A a → Deriv e (Γl.cons ⟨A, ⊤, ⊥⟩) B b → Deriv e Γ B (.let₁ a A b)
   | unit {Γ} : Γ.Wk .nil → Deriv e Γ .unit .unit
   | pair {Γ Γl Γr e A B a b} :
     Γ.PSSplit Γl Γr →
     Deriv e Γl A a → Deriv e Γr B b → Deriv e Γ (.tensor A B) (.pair a b)
   | let₂ {Γ Γl Γr e A B C a b} :
-    Γ.PSSplit Γr Γl →
-    Deriv e Γl (.tensor A B) a → Deriv e ((Γr.cons ⟨A, ⊤, ⊥⟩).cons ⟨B, ⊤, ⊥⟩) C b
+    Γ.PSSplit Γl Γr →
+    Deriv e Γr (.tensor A B) a → Deriv e ((Γl.cons ⟨A, ⊤, ⊥⟩).cons ⟨B, ⊤, ⊥⟩) C b
       → Deriv e Γ C (.let₂ a A B b)
   | inl {Γ e A B a} : Deriv e Γ A a → Deriv e Γ (.coprod A B) (.inl A B a)
   | inr {Γ e A B b} : Deriv e Γ B b → Deriv e Γ (.coprod A B) (.inr A B b)
@@ -32,10 +32,10 @@ inductive Deriv : ε → Ctx? α ε → Ty α → Term φ (Ty α) → Type _
       → Deriv e Γ C (.case a A B b c)
   | abort {Γ e A a} : Deriv e Γ .empty a → Deriv e Γ A (.abort A a)
   | iter {Γ Γl Γr e A B a b} :
-    Γ.PSSplit Γr Γl →
+    Γ.PSSplit Γl Γr →
     e ∈ S.iterative →
-    Γr.copy → Γr.del →
-    Deriv e Γl A a → Deriv e (Γr.cons ⟨A, ⊤, ⊥⟩) (.coprod B A) b → Deriv e Γ B (.iter a A B b)
+    Γl.copy → Γl.del →
+    Deriv e Γr A a → Deriv e (Γl.cons ⟨A, ⊤, ⊥⟩) (.coprod B A) b → Deriv e Γ B (.iter a A B b)
 
 notation Γ "⊢[" e "]" a ":" A => Deriv e Γ A a
 
@@ -56,3 +56,193 @@ def Deriv.mono {e e' : ε} {Γ : Ctx? α ε} {A : Ty α} {a : Term φ (Ty α)} (
 
 abbrev Deriv.top {e : ε} {Γ : Ctx? α ε} {A : Ty α} {a : Term φ (Ty α)}
   (D : Γ ⊢[e] a : A) : (Γ ⊢[⊤] a : A) := D.mono le_top
+
+def Deriv.cast {e e' : ε} {Γ Γ' : Ctx? α ε} {A A' : Ty α} {a a' : Term φ (Ty α)}
+  (he : e = e') (hΓ : Γ = Γ') (hA : A = A') (ha : a = a')
+  (D : Γ ⊢[e] a : A) : (Γ' ⊢[e'] a' : A') := he ▸ hΓ ▸ hA ▸ ha ▸ D
+
+abbrev Deriv.cast_eff {e e' : ε} {Γ : Ctx? α ε} {A : Ty α} {a : Term φ (Ty α)}
+  (he : e = e') (D : Γ ⊢[e] a : A) : Γ ⊢[e'] a : A := D.cast he rfl rfl rfl
+
+abbrev Deriv.cast_ctx {e : ε} {Γ Γ' : Ctx? α ε} {A : Ty α} {a : Term φ (Ty α)}
+  (hΓ : Γ = Γ') (D : Γ ⊢[e] a : A) : Γ' ⊢[e] a : A := D.cast rfl hΓ rfl rfl
+
+abbrev Deriv.cast_ty {e : ε} {Γ : Ctx? α ε} {A A' : Ty α} {a : Term φ (Ty α)}
+  (hA : A = A') (D : Γ ⊢[e] a : A) : Γ ⊢[e] a : A' := D.cast rfl rfl hA rfl
+
+abbrev Deriv.cast_term {e : ε} {Γ : Ctx? α ε} {A : Ty α} {a a' : Term φ (Ty α)}
+  (ha : a = a') (D : Γ ⊢[e] a : A) : Γ ⊢[e] a' : A := D.cast rfl rfl rfl ha
+
+def IsWt (e : ε) (Γ : Ctx? α ε) (A : Ty α) (a : Term φ (Ty α)) : Prop := Nonempty (Γ ⊢[e] a : A)
+
+@[match_pattern]
+theorem Deriv.wt {e : ε} {Γ : Ctx? α ε} {A : Ty α} {a : Term φ (Ty α)} (D : Γ ⊢[e] a : A)
+  : IsWt e Γ A a := ⟨D⟩
+
+theorem IsWt.mono {e e' : ε} {Γ : Ctx? α ε} {A : Ty α} {a : Term φ (Ty α)} (he : e ≤ e')
+  : IsWt e Γ A a → IsWt e' Γ A a := λ ⟨D⟩ => ⟨D.mono he⟩
+
+theorem IsWt.top {e : ε} {Γ : Ctx? α ε} {A : Ty α} {a : Term φ (Ty α)}
+  (D : IsWt e Γ A a) : IsWt ⊤ Γ A a := D.mono le_top
+
+theorem Deriv.wt_top {e : ε} {Γ : Ctx? α ε} {A : Ty α} {a : Term φ (Ty α)} (D : Γ ⊢[e] a : A)
+  : IsWt ⊤ Γ A a := D.wt.top
+
+theorem IsWt.exists_iff {Γ : Ctx? α ε} {A : Ty α} {a : Term φ (Ty α)}
+  : (∃e, IsWt e Γ A a) ↔ IsWt ⊤ Γ A a := ⟨λ⟨_, h⟩ => h.top, λh => ⟨⊤, h⟩⟩
+
+theorem Deriv.bv_at {e : ε} {Γ : Ctx? α ε} {A : Ty α} {n : ℕ} (D : Γ ⊢[e] (.bv (φ := φ) n) : A)
+  : Γ.At ⟨A, 1, e⟩ n := match D with | .bv hv => hv
+
+theorem IsWt.bv_at {e : ε} {Γ : Ctx? α ε} {A : Ty α} {n : ℕ} (D : IsWt (φ := φ) e Γ A (.bv n))
+  : Γ.At ⟨A, 1, e⟩ n := D.elim Deriv.bv_at
+
+theorem Deriv.op_fn {e : ε} {Γ : Ctx? α ε} {B : Ty α} {f : φ} {a : Term φ (Ty α)}
+  (D : Γ ⊢[e] (.op f a) : B) : S.IsFn f e (S.src f) B
+  := match D with | .op hf da => by cases hf.src; exact hf
+
+theorem IsWt.op_fn {e : ε} {Γ : Ctx? α ε} {B : Ty α} {f : φ} {a : Term φ (Ty α)}
+  (D : IsWt e Γ B (.op f a)) : S.IsFn f e (S.src f) B := D.elim Deriv.op_fn
+
+def Deriv.op_arg {e : ε} {Γ : Ctx? α ε} {B : Ty α} {f : φ} {a : Term φ (Ty α)}
+  (D : Γ ⊢[e] (.op f a) : B) : Γ ⊢[e] a : S.src f
+  := match D with | .op hf da => da.cast_ty hf.src
+
+theorem IsWt.op_arg {e : ε} {Γ : Ctx? α ε} {B : Ty α} {f : φ} {a : Term φ (Ty α)}
+  (D : IsWt e Γ B (.op f a)) : IsWt e Γ (S.src f) a := ⟨(Classical.choice D).op_arg⟩
+
+def Deriv.let₁_splitLeft {e : ε} {Γ : Ctx? α ε} {A B : Ty α} {a b : Term φ (Ty α)}
+  (D : Γ ⊢[e] (.let₁ a A b) : B) : Ctx? α ε
+  := match D with | .let₁ (Γl := Γl) .. => Γl
+
+def Deriv.let₁_splitRight {e : ε} {Γ : Ctx? α ε} {A B : Ty α} {a b : Term φ (Ty α)}
+  (D : Γ ⊢[e] (.let₁ a A b) : B) : Ctx? α ε
+  := match D with | .let₁ (Γr := Γr) .. => Γr
+
+def Deriv.let₁_split {e : ε} {Γ : Ctx? α ε} {A B : Ty α} {a b : Term φ (Ty α)}
+  (D : Γ ⊢[e] (.let₁ a A b) : B) : Γ.PSSplit (D.let₁_splitLeft) (D.let₁_splitRight)
+  := match D with | .let₁ dΓ _ _ => dΓ
+
+def Deriv.let₁_bind {e : ε} {Γ : Ctx? α ε} {A B : Ty α} {a b : Term φ (Ty α)}
+  (D : Γ ⊢[e] (.let₁ a A b) : B) : D.let₁_splitRight ⊢[e] a : A
+  := match D with | .let₁ _ da _ => da
+
+def Deriv.let₁_expr {e : ε} {Γ : Ctx? α ε} {A B : Ty α} {a b : Term φ (Ty α)}
+  (D : Γ ⊢[e] (.let₁ a A b) : B) : (D.let₁_splitLeft.cons ⟨A, ⊤, ⊥⟩) ⊢[e] b : B
+  := match D with | .let₁ _ _ db => db
+
+def Deriv.unit_wk {e : ε} {Γ : Ctx? α ε} (D : Γ ⊢[e] .unit (φ := φ) : .unit) : Γ.Wk .nil
+  := match D with | .unit dΓ => dΓ
+
+def Deriv.pair_splitLeft {e : ε} {Γ : Ctx? α ε} {A B : Ty α} {a b : Term φ (Ty α)}
+  (D : Γ ⊢[e] (.pair a b) : .tensor A B) : Ctx? α ε
+  := match D with | .pair (Γl := Γl) .. => Γl
+
+def Deriv.pair_splitRight {e : ε} {Γ : Ctx? α ε} {A B : Ty α} {a b : Term φ (Ty α)}
+  (D : Γ ⊢[e] (.pair a b) : .tensor A B) : Ctx? α ε
+  := match D with | .pair (Γr := Γr) .. => Γr
+
+def Deriv.pair_split {e : ε} {Γ : Ctx? α ε} {A B : Ty α} {a b : Term φ (Ty α)}
+  (D : Γ ⊢[e] (.pair a b) : .tensor A B) : Γ.PSSplit (D.pair_splitLeft) (D.pair_splitRight)
+  := match D with | .pair dΓ _ _ => dΓ
+
+def Deriv.pair_left {e : ε} {Γ : Ctx? α ε} {A B : Ty α} {a b : Term φ (Ty α)}
+  (D : Γ ⊢[e] (.pair a b) : .tensor A B) : D.pair_splitLeft ⊢[e] a : A
+  := match D with | .pair _ da _ => da
+
+def Deriv.pair_right {e : ε} {Γ : Ctx? α ε} {A B : Ty α} {a b : Term φ (Ty α)}
+  (D : Γ ⊢[e] (.pair a b) : .tensor A B) : D.pair_splitRight ⊢[e] b : B
+  := match D with | .pair _ _ db => db
+
+def Deriv.let₂_splitLeft {e : ε} {Γ : Ctx? α ε} {A B C : Ty α} {a b : Term φ (Ty α)}
+  (D : Γ ⊢[e] (.let₂ a A B b) : C) : Ctx? α ε
+  := match D with | .let₂ (Γl := Γl) .. => Γl
+
+def Deriv.let₂_splitRight {e : ε} {Γ : Ctx? α ε} {A B C : Ty α} {a b : Term φ (Ty α)}
+  (D : Γ ⊢[e] (.let₂ a A B b) : C) : Ctx? α ε
+  := match D with | .let₂ (Γr := Γr) .. => Γr
+
+def Deriv.let₂_split {e : ε} {Γ : Ctx? α ε} {A B C : Ty α} {a b : Term φ (Ty α)}
+  (D : Γ ⊢[e] (.let₂ a A B b) : C) : Γ.PSSplit (D.let₂_splitLeft) (D.let₂_splitRight)
+  := match D with | .let₂ dΓ _ _ => dΓ
+
+def Deriv.let₂_bind {e : ε} {Γ : Ctx? α ε} {A B C : Ty α} {a b : Term φ (Ty α)}
+  (D : Γ ⊢[e] (.let₂ a A B b) : C) : D.let₂_splitRight ⊢[e] a : .tensor A B
+  := match D with | .let₂ _ da _ => da
+
+def Deriv.let₂_expr {e : ε} {Γ : Ctx? α ε} {A B C : Ty α} {a b : Term φ (Ty α)}
+  (D : Γ ⊢[e] (.let₂ a A B b) : C) : (D.let₂_splitLeft.cons ⟨A, ⊤, ⊥⟩).cons ⟨B, ⊤, ⊥⟩ ⊢[e] b : C
+  := match D with | .let₂ _ _ db => db
+
+def Deriv.inl_arg {e : ε} {Γ : Ctx? α ε} {A B : Ty α} {a : Term φ (Ty α)}
+  (D : Γ ⊢[e] (.inl A B a) : .coprod A B) : Γ ⊢[e] a : A
+  := match D with | .inl da => da
+
+def Deriv.inr_arg {e : ε} {Γ : Ctx? α ε} {A B : Ty α} {b : Term φ (Ty α)}
+  (D : Γ ⊢[e] (.inr A B b) : .coprod A B) : Γ ⊢[e] b : B
+  := match D with | .inr db => db
+
+def Deriv.case_splitLeft {e : ε} {Γ : Ctx? α ε} {A B C : Ty α} {a b c : Term φ (Ty α)}
+  (D : Γ ⊢[e] (.case a A B b c) : C) : Ctx? α ε
+  := match D with | .case (Γl := Γl) .. => Γl
+
+def Deriv.case_splitRight {e : ε} {Γ : Ctx? α ε} {A B C : Ty α} {a b c : Term φ (Ty α)}
+  (D : Γ ⊢[e] (.case a A B b c) : C) : Ctx? α ε
+  := match D with | .case (Γr := Γr) .. => Γr
+
+def Deriv.case_bind {e : ε} {Γ : Ctx? α ε} {A B C : Ty α} {a b c : Term φ (Ty α)}
+  (D : Γ ⊢[e] (.case a A B b c) : C) : D.case_splitRight ⊢[e] a : .coprod A B
+  := match D with | .case _ da _ _ => da
+
+def Deriv.case_left {e : ε} {Γ : Ctx? α ε} {A B C : Ty α} {a b c : Term φ (Ty α)}
+  (D : Γ ⊢[e] (.case a A B b c) : C) : D.case_splitLeft.cons ⟨A, ⊤, ⊥⟩ ⊢[e] b : C
+  := match D with | .case _ _ db _ => db
+
+def Deriv.case_right {e : ε} {Γ : Ctx? α ε} {A B C : Ty α} {a b c : Term φ (Ty α)}
+  (D : Γ ⊢[e] (.case a A B b c) : C) : D.case_splitLeft.cons ⟨B, ⊤, ⊥⟩ ⊢[e] c : C
+  := match D with | .case _ _ _ dc => dc
+
+def Deriv.abort_arg {e : ε} {Γ : Ctx? α ε} {A : Ty α} {a : Term φ (Ty α)}
+  (D : Γ ⊢[e] (.abort A a) : A) : Γ ⊢[e] a : .empty
+  := match D with | .abort da => da
+
+def Deriv.iter_splitLeft {e : ε} {Γ : Ctx? α ε} {A B : Ty α} {a b : Term φ (Ty α)}
+  (D : Γ ⊢[e] (.iter a A B b) : B) : Ctx? α ε
+  := match D with | .iter (Γl := Γl) .. => Γl
+
+def Deriv.iter_splitRight {e : ε} {Γ : Ctx? α ε} {A B : Ty α} {a b : Term φ (Ty α)}
+  (D : Γ ⊢[e] (.iter a A B b) : B) : Ctx? α ε
+  := match D with | .iter (Γr := Γr) .. => Γr
+
+def Deriv.iter_split {e : ε} {Γ : Ctx? α ε} {A B : Ty α} {a b : Term φ (Ty α)}
+  (D : Γ ⊢[e] (.iter a A B b) : B) : Γ.PSSplit (D.iter_splitLeft) (D.iter_splitRight)
+  := match D with | .iter dΓ _ _ _ _ _ => dΓ
+
+theorem Deriv.iter_eff {e : ε} {Γ : Ctx? α ε} {A B : Ty α} {a b : Term φ (Ty α)}
+  (D : Γ ⊢[e] (.iter a A B b) : B) : e ∈ S.iterative
+  := match D with | .iter _ hei _ _ _ _ => hei
+
+theorem IsWt.iter_eff {e : ε} {Γ : Ctx? α ε} {A B : Ty α} {a b : Term φ (Ty α)}
+  (D : IsWt e Γ B (.iter a A B b)) : e ∈ S.iterative := D.elim Deriv.iter_eff
+
+theorem Deriv.iter_copy {e : ε} {Γ : Ctx? α ε} {A B : Ty α} {a b : Term φ (Ty α)}
+  (D : Γ ⊢[e] (.iter a A B b) : B) : D.iter_splitLeft.copy
+  := match D with | .iter _ _ hc _ _ _ => hc
+
+theorem Deriv.iter_del {e : ε} {Γ : Ctx? α ε} {A B : Ty α} {a b : Term φ (Ty α)}
+  (D : Γ ⊢[e] (.iter a A B b) : B) : D.iter_splitLeft.del
+  := match D with | .iter _ _ _ hd _ _ => hd
+
+def Deriv.iter_bind {e : ε} {Γ : Ctx? α ε} {A B : Ty α} {a b : Term φ (Ty α)}
+  (D : Γ ⊢[e] (.iter a A B b) : B) : D.iter_splitRight ⊢[e] a : A
+  := match D with | .iter _ _ _ _ da _ => da
+
+def Deriv.iter_iter {e : ε} {Γ : Ctx? α ε} {A B : Ty α} {a b : Term φ (Ty α)}
+  (D : Γ ⊢[e] (.iter a A B b) : B) : D.iter_splitLeft.cons ⟨A, ⊤, ⊥⟩ ⊢[e] b : .coprod B A
+  := match D with | .iter _ _ _ _ _ db => db
+
+--TODO: want minimization for IsWt inversion...
+
+end Term
+
+end Refinery
