Refinery/Ctx/Add.lean
@@ -1,0 +1,49 @@
+import Refinery.Ctx.Basic
+
+namespace Refinery
+
+def Var?.add (v w : Var? α ε) : Var? α ε := ⟨v.ty, v.q + w.q, v.eff⟩
+
+instance Var?.instAdd : Add (Var? α ε) where
+  add := Var?.add
+
+theorem Var?.add_def (v w : Var? α ε) : v + w = ⟨v.ty, v.q + w.q, v.eff⟩ := rfl
+
+@[simp]
+theorem Var?.add_erase (v : Var? α ε) : v + v.erase = v := by simp [add_def]
+
+@[simp]
+theorem Var?.erase_add (v : Var? α ε) : v.erase + v = v := by simp [add_def]
+
+instance Var?.instAddSemigroup : AddSemigroup (Var? α ε) where
+  add_assoc u v w := by simp [Var?.add_def, add_assoc]
+
+def Ctx?.add (Γ Δ : Ctx? α ε) : Ctx? α ε := match Γ, Δ with
+  | .nil, Δ => Δ
+  | Γ, .nil => Γ
+  | .cons Γ v, .cons Δ w => .cons (Γ.add Δ) (v + w)
+
+instance Ctx?.instAdd : Add (Ctx? α ε) where
+  add := Ctx?.add
+
+@[simp]
+theorem Ctx?.add_nil (Γ : Ctx? α ε) : Γ + .nil = Γ := by cases Γ <;> rfl
+
+@[simp]
+theorem Ctx?.nil_add (Γ : Ctx? α ε) : .nil + Γ = Γ := by cases Γ <;> rfl
+
+@[simp]
+theorem Ctx?.cons_add_cons (Γ Δ : Ctx? α ε) (v w : Var? α ε)
+  : Γ.cons v + Δ.cons w = .cons (Γ + Δ) (v + w) := rfl
+
+@[simp]
+theorem Ctx?.add_erase (Γ : Ctx? α ε) : Γ + Γ.erase = Γ := by induction Γ <;> simp [*]
+
+instance Ctx?.instZero : Zero (Ctx? α ε) where
+  zero := .nil
+
+instance AddMonoid : AddMonoid (Ctx? α ε) where
+  add_assoc Γ Δ Ξ := by induction Γ generalizing Δ Ξ <;> cases Δ <;> cases Ξ <;> simp [add_assoc, *]
+  zero_add Γ := Γ.nil_add
+  add_zero Γ := Γ.add_nil
+  nsmul := nsmulRec
